Various tweaks for LTL (6). (#48)
* pattern_interpretation_exists_of_sort_predicate

* M_predicate_forall_of_sort

* WIP

* type classes for syntax

* fix and use simpl_evar_open.

* simpl_svar_open, Definedness instancess

src/Syntax.v
@@ -75,7 +75,6 @@ Section syntax.
     - apply nat_eq_dec.
     - apply sym_eq.
   Qed.
-      
 
   Definition Theory := Ensemble Pattern.
   
@@ -295,7 +294,7 @@ Section syntax.
     | patt_exists p' => patt_exists (evar_open (k + 1) n p')
     | patt_mu p' => patt_mu (evar_open k n p')
     end.
-
+  
   (* The following lemmas are trivial but useful for autorewrite. *)
   Lemma evar_open_free_evar k n x: evar_open k n (patt_free_evar x) = patt_free_evar x.
   Proof. reflexivity. Qed.
@@ -355,6 +354,110 @@ Section syntax.
   Proof. reflexivity. Qed.
   Lemma svar_open_mu k n p': svar_open k n (patt_mu p') = patt_mu (svar_open (k + 1) n p').
   Proof. reflexivity. Qed.
+
+
+  (* TODO free_evars, free_svars *)
+  Class EBinder (ebinder : Pattern -> Pattern) :=
+    {
+      ebinder_evar_open :
+        forall k n ϕ, evar_open k n (ebinder ϕ) = ebinder (evar_open (k + 1) n ϕ) ;
+      ebinder_svar_open :
+        forall k n ϕ, svar_open k n (ebinder ϕ) = ebinder (svar_open k n ϕ) ;
+    }.
+
+  Class SBinder (sbinder : Pattern -> Pattern) :=
+    {
+      sbinder_evar_open :
+        forall k n ϕ, evar_open k n (sbinder ϕ) = sbinder (evar_open k n ϕ) ;
+      sbinder_svar_open :
+        forall k n ϕ, svar_open k n (sbinder ϕ) = sbinder (svar_open (k + 1) n ϕ) ;
+    }.
+
+  (* Non-variable nullary operation *)
+  Class NVNullary (nvnullary : Pattern) :=
+    {
+      nvnullary_evar_open :
+        forall k n, evar_open k n nvnullary = nvnullary ;
+      nvnullary_svar_open :
+        forall k n, svar_open k n nvnullary = nvnullary ;
+    }.
+
+  Class Unary (patt : Pattern -> Pattern) :=
+    {
+      unary_evar_open :
+        forall k n ϕ, evar_open k n (patt ϕ) = patt (evar_open k n ϕ) ;
+      unary_svar_open :
+        forall k n ϕ, svar_open k n (patt ϕ) = patt (svar_open k n ϕ) ;
+    }.
+
+  Class Binary (binary : Pattern -> Pattern -> Pattern) :=
+    {
+      binary_evar_open :
+        forall k n ϕ₁ ϕ₂, evar_open k n (binary ϕ₁ ϕ₂) = binary (evar_open k n ϕ₁) (evar_open k n ϕ₂) ;
+      binary_svar_open :
+        forall k n ϕ₁ ϕ₂, svar_open k n (binary ϕ₁ ϕ₂) = binary (svar_open k n ϕ₁) (svar_open k n ϕ₂) ;
+    }.
+
+  (* TODO the same for svar_open *)
+  Definition simpl_evar_open :=
+    (@ebinder_evar_open,
+     @sbinder_evar_open,
+     @nvnullary_evar_open,
+     @unary_evar_open,
+     @binary_evar_open
+    ).
+
+  Definition simpl_svar_open :=
+    (@ebinder_svar_open,
+     @sbinder_svar_open,
+     @nvnullary_svar_open,
+     @unary_svar_open,
+     @binary_svar_open
+    ).
+  
+
+  #[global]
+  Instance EBinder_exists : EBinder patt_exists :=
+    {|
+       ebinder_evar_open := evar_open_exists ;
+       ebinder_svar_open := svar_open_exists ;
+    |}.
+
+  #[global]
+  Instance SBinder_mu : SBinder patt_mu :=
+    {|
+       sbinder_evar_open := evar_open_mu ;
+       sbinder_svar_open := svar_open_mu ;
+    |}.
+
+
+  #[global]
+  Instance NVNullary_bott : NVNullary patt_bott :=
+    {|
+       nvnullary_evar_open := evar_open_bott ;
+       nvnullary_svar_open := svar_open_bott ;
+    |}.
+
+  #[global]
+  Instance NVNullary_sym s : NVNullary (patt_sym s) :=
+    {|
+       nvnullary_evar_open := λ k n, @evar_open_sym k n s ;
+       nvnullary_svar_open := λ k n, @svar_open_sym k n s ;
+    |}.
+
+  #[global]
+  Instance Binary_app : Binary patt_app :=
+    {|
+       binary_evar_open := evar_open_app ;
+       binary_svar_open := svar_open_app ;
+    |}.
+
+  #[global]
+  Instance Binary_imp : Binary patt_imp :=
+    {|
+       binary_evar_open := evar_open_imp ;
+       binary_svar_open := svar_open_imp ;
+    |}.
   
   Lemma evar_open_size :
     forall (k : db_index) (n : evar) (p : Pattern),
@@ -1305,6 +1408,49 @@ Section syntax.
   Lemma svar_open_forall k x ϕ : svar_open k x (patt_forall ϕ) = patt_forall (svar_open k x ϕ).
   Proof. simpl. unfold patt_forall. unfold patt_not. reflexivity. Qed.
 
+  #[global]
+  Instance Unary_not : Unary patt_not :=
+    {|
+       unary_evar_open := evar_open_not ;
+       unary_svar_open := svar_open_not ;
+    |}.
+
+  #[global]
+  Instance NVNullary_top : NVNullary patt_top :=
+    {|
+       nvnullary_evar_open := evar_open_top ;
+       nvnullary_svar_open := svar_open_top ;
+    |}.
+
+  #[global]
+  Instance Binary_or : Binary patt_or :=
+    {|
+       binary_evar_open := evar_open_or ;
+       binary_svar_open := svar_open_or ;
+    |}.
+
+  #[global]
+  Instance Binary_and : Binary patt_and :=
+    {|
+       binary_evar_open := evar_open_and ;
+       binary_svar_open := svar_open_and ;
+    |}.
+
+  #[global]
+  Instance Binary_iff : Binary patt_iff :=
+    {|
+       binary_evar_open := evar_open_iff ;
+       binary_svar_open := svar_open_iff ;
+    |}.
+
+  #[global]
+  Instance EBinder_forall : EBinder patt_forall :=
+    {|
+       ebinder_evar_open := evar_open_forall ;
+       ebinder_svar_open := svar_open_forall ;
+    |}.
+
+  
   Lemma free_svars_svar_open ϕ X dbi :
     free_svars (svar_open dbi X ϕ) ⊆ union (singleton X) (free_svars ϕ).
   Proof.
