src/Theories/Sorts.v
@@ -6,6 +6,8 @@ Unset Printing Implicit Defensive.
 From Coq Require Import Unicode.Utf8.
 From Coq.Logic Require Import Classical_Prop FunctionalExtensionality.
 
+From stdpp Require Import base.
+
 From MatchingLogic Require Import Syntax Semantics.
 Require Import MatchingLogic.Theories.Definedness.
 
@@ -59,21 +61,26 @@ Section sorts.
     (* ϕ is expected to be a sort pattern *)
     Definition Minterp_inhabitant ϕ ρₑ ρₛ := @pattern_interpretation sig M ρₑ ρₛ (patt_app (sym inhabitant) ϕ).
 
-    Lemma pattern_interpretation_forall_of_sort_predicate s ϕ ρₑ ρₛ:
-      (* s is closed *)
-      free_evars s = base.empty ->
-      well_formed_closed s ->
+
+    Class PSort :=
+      { patt_sort : Pattern ;
+        patt_sort_closed : free_evars patt_sort = ∅ ;
+        patt_sort_wfc : well_formed_closed patt_sort ;
+      }.
+    
+    
+    Lemma pattern_interpretation_forall_of_sort_predicate (s : PSort) ϕ ρₑ ρₛ:
       let x := fresh_evar ϕ in
       M_predicate M (evar_open 0 x ϕ) ->
-      pattern_interpretation ρₑ ρₛ (patt_forall_of_sort s ϕ) = Full
-      <-> (∀ m : Domain M, Minterp_inhabitant s ρₑ ρₛ m ->
+      pattern_interpretation ρₑ ρₛ (patt_forall_of_sort (@patt_sort s) ϕ) = Full
+      <-> (∀ m : Domain M, Minterp_inhabitant (@patt_sort s) ρₑ ρₛ m ->
                            pattern_interpretation (update_evar_val x m ρₑ) ρₛ (evar_open 0 x ϕ) = Full).
     Proof.
-      intros Hs Hwfc x Hpred.
+      intros x Hpred.
       unfold patt_forall_of_sort.
-      assert (Hfr: fresh_evar (patt_in b0 (inhabitant_set s) ---> ϕ) = fresh_evar ϕ).
+      assert (Hfr: fresh_evar (patt_in b0 (inhabitant_set patt_sort) ---> ϕ) = fresh_evar ϕ).
       { unfold fresh_evar. apply f_equal. apply f_equal. simpl.
-        rewrite -> Hs.
+        rewrite -> patt_sort_closed.
         repeat rewrite -> sets.union_empty_l_L.
         auto.
       }
@@ -96,16 +103,16 @@ Section sorts.
         rewrite -> Hfr in H.
         eapply pattern_interpretation_impl_MP. apply H.
         unfold Minterp_inhabitant in H'.
-        pose proof (Hfeip := free_evar_in_patt M M_satisfies_theory (fresh_evar ϕ) (patt_sym (inj inhabitant) $ evar_open 0 (fresh_evar ϕ) s) (update_evar_val (fresh_evar ϕ) m ρₑ) ρₛ).
+        pose proof (Hfeip := @free_evar_in_patt _ _ M M_satisfies_theory (fresh_evar ϕ) (patt_sym (inj inhabitant) $ evar_open 0 (fresh_evar ϕ) patt_sort) (update_evar_val (fresh_evar ϕ) m ρₑ) ρₛ).
         destruct Hfeip as [Hfeip1 _]. apply Hfeip1. clear Hfeip1.
         rewrite update_evar_val_same.
         clear H. unfold sym in H'.
         unfold Ensembles.In.
-        rewrite -> evar_open_wfc. 2: apply Hwfc.
+        rewrite -> evar_open_wfc. 2: apply patt_sort_wfc.
         rewrite -> pattern_interpretation_free_evar_independent.
         3: { intros Contra. simpl in Contra.
              rewrite -> sets.union_empty_l_L in Contra.
-             rewrite -> Hs in Contra.
+             rewrite -> patt_sort_closed in Contra.
              apply base.not_elem_of_empty in Contra.
              apply Contra.
         }
@@ -113,12 +120,12 @@ Section sorts.
              constructor.
              constructor.
              apply wfc_wfc_ind.
-             apply Hwfc.
+             apply patt_sort_wfc.
         }
         apply H'.
       - intros H m.
         autorewrite with ml_db. simpl.
-        pose proof (Hfeip := free_evar_in_patt M M_satisfies_theory (fresh_evar ϕ) (patt_sym (inj inhabitant) $ evar_open 0 (fresh_evar ϕ) s) (update_evar_val (fresh_evar ϕ) m ρₑ) ρₛ).
+        pose proof (Hfeip := @free_evar_in_patt _ _ M M_satisfies_theory (fresh_evar ϕ) (patt_sym (inj inhabitant) $ evar_open 0 (fresh_evar ϕ) patt_sort) (update_evar_val (fresh_evar ϕ) m ρₑ) ρₛ).
         destruct Hfeip as [_ Hfeip2].
         apply pattern_interpretation_predicate_impl.
         apply T_predicate_in. apply M_satisfies_theory.
@@ -126,12 +133,12 @@ Section sorts.
         specialize (Hfeip2 H1). clear H1.
         apply H. unfold Minterp_inhabitant.
         unfold Ensembles.In in Hfeip2. unfold sym.
-        rewrite -> evar_open_wfc in Hfeip2. 2: apply Hwfc.
+        rewrite -> evar_open_wfc in Hfeip2. 2: apply patt_sort_wfc.
         rewrite -> update_evar_val_same in Hfeip2.
         rewrite -> pattern_interpretation_free_evar_independent in Hfeip2.
         3: { intros Contra. simpl in Contra.
              rewrite -> sets.union_empty_l_L in Contra.
-             rewrite -> Hs in Contra.
+             rewrite -> patt_sort_closed in Contra.
              apply base.not_elem_of_empty in Contra.
              apply Contra.
         }
@@ -139,22 +146,151 @@ Section sorts.
              constructor.
              constructor.
              apply wfc_wfc_ind.
-             apply Hwfc.
+             apply patt_sort_wfc.
         }
         apply Hfeip2.
     Qed.
+
+    Lemma pattern_interpretation_exists_of_sort_predicate (s : PSort) ϕ ρₑ ρₛ:
+      let x := fresh_evar ϕ in
+      M_predicate M (evar_open 0 x ϕ) ->
+      pattern_interpretation ρₑ ρₛ (patt_exists_of_sort patt_sort ϕ) = Full
+      <-> (∃ m : Domain M, Minterp_inhabitant patt_sort ρₑ ρₛ m /\
+                           pattern_interpretation (update_evar_val x m ρₑ) ρₛ (evar_open 0 x ϕ) = Full).
+    Proof.
+      intros x Hpred.
+      unfold patt_exists_of_sort.
+      assert (Hfr: fresh_evar (patt_in b0 (inhabitant_set patt_sort) and ϕ) = fresh_evar ϕ).
+      { unfold fresh_evar. apply f_equal. apply f_equal. simpl.
+        rewrite -> patt_sort_closed.
+        repeat rewrite -> sets.union_empty_r_L.
+        rewrite -> sets.union_empty_l_L.
+        auto.
+      }
+      rewrite -> pattern_interpretation_exists_predicate_full.
+      2: {
+        autorewrite with ml_db.
+        simpl.
+        apply M_predicate_and.
+        - apply T_predicate_in.
+          apply M_satisfies_theory.
+        - subst x.
+          rewrite -> Hfr.
+          apply Hpred.
+      }
+      subst x.
+      split.
+      - intros [m H].
+        autorewrite with ml_db in H. simpl in H.
+        rewrite -> Hfr in H.
+        apply pattern_interpretation_and_full in H.
+        destruct H as [H1 H2].
+        exists m. split. 2: apply H2. clear H2.
+        unfold Minterp_inhabitant.
+        pose proof (Hfeip := @free_evar_in_patt _ _ M M_satisfies_theory (fresh_evar ϕ) (patt_sym (inj inhabitant) $ evar_open 0 (fresh_evar ϕ) patt_sort) (update_evar_val (fresh_evar ϕ) m ρₑ) ρₛ).
+        destruct Hfeip as [_ Hfeip2]. apply Hfeip2 in H1. clear Hfeip2.
+        rewrite update_evar_val_same in H1.
+        unfold sym.
+        unfold Ensembles.In in H1.
+        rewrite -> evar_open_wfc in H1. 2: apply patt_sort_wfc.
+        rewrite -> pattern_interpretation_free_evar_independent in H1.
+        3: { intros Contra. simpl in Contra.
+             rewrite -> sets.union_empty_l_L in Contra.
+             rewrite -> patt_sort_closed in Contra.
+             apply base.not_elem_of_empty in Contra.
+             apply Contra.
+        }
+        2: { apply wfc_ind_wfc.
+             constructor.
+             constructor.
+             apply wfc_wfc_ind.
+             apply patt_sort_wfc.
+        }
+        apply H1.
+      - intros [m [H1 H2]]. exists m.
+        autorewrite with ml_db. simpl.
+        pose proof (Hfeip := @free_evar_in_patt _ _ M M_satisfies_theory (fresh_evar ϕ) (patt_sym (inj inhabitant) $ evar_open 0 (fresh_evar ϕ) patt_sort) (update_evar_val (fresh_evar ϕ) m ρₑ) ρₛ).
+        destruct Hfeip as [Hfeip1 _].
+        apply pattern_interpretation_and_full.
+        rewrite -> Hfr.
+        split.
+        + apply Hfeip1. clear Hfeip1.
+          unfold Ensembles.In.
+          rewrite -> update_evar_val_same.
+          unfold Minterp_inhabitant in H1. unfold sym in H1.
+          rewrite -> evar_open_wfc. 2: apply patt_sort_wfc.
+          rewrite -> pattern_interpretation_free_evar_independent.
+          3: { intros Contra. simpl in Contra.
+               rewrite -> sets.union_empty_l_L in Contra.
+               rewrite -> patt_sort_closed in Contra.
+               apply base.not_elem_of_empty in Contra.
+               apply Contra.
+          }
+          2: { apply wfc_ind_wfc.
+               constructor.
+               constructor.
+               apply wfc_wfc_ind.
+               apply patt_sort_wfc.
+          }
+          apply H1.
+        + apply H2.
+    Qed.
+
+
+    Lemma M_predicate_exists_of_sort (s : PSort) ϕ :
+      let x := fresh_evar ϕ in
+      M_predicate M (evar_open 0 x ϕ) -> M_predicate M (patt_exists_of_sort patt_sort ϕ).
+    Proof.
+      intros x Hpred.
+      unfold patt_exists_of_sort.
+      apply M_predicate_exists.
+      autorewrite with ml_db. rewrite [if PeanoNat.Nat.eqb 0 0 then _ else _]/=.
+      apply M_predicate_and.
+      - apply T_predicate_in.
+        apply M_satisfies_theory.
+      - simpl.
+        rewrite -> patt_sort_closed.
+        repeat rewrite sets.union_empty_r_L.
+        repeat rewrite sets.union_empty_l_L.
+        subst x.
+        unfold fresh_evar in Hpred.
+        apply Hpred.
+    Qed.
+
+    Lemma M_predicate_forall_of_sort (s : PSort) ϕ :
+      let x := fresh_evar ϕ in
+      M_predicate M (evar_open 0 x ϕ) -> M_predicate M (patt_forall_of_sort patt_sort ϕ).
+    Proof.
+      intros x Hpred.
+      unfold patt_forall_of_sort.
+      apply M_predicate_forall.
+      autorewrite with ml_db. rewrite [if PeanoNat.Nat.eqb 0 0 then _ else _]/=.
+      apply M_predicate_impl.
+      - apply T_predicate_in.
+        apply M_satisfies_theory.
+      - simpl.
+        rewrite -> patt_sort_closed.
+        rewrite !(@right_id _ (=) ∅ (∪) ).
+        rewrite (@left_id _ (=) ∅).
+        subst x.
+        unfold fresh_evar in Hpred.
+        apply Hpred.
+    Qed.
+
     
-    Lemma interp_total_function f s₁ s₂ ρₑ ρₛ :
-      @pattern_interpretation sig M ρₑ ρₛ (patt_total_function f s₁ s₂) = Full ->
+    Lemma interp_total_function f (s₁ s₂ : PSort) ρₑ ρₛ :
+      @pattern_interpretation sig M ρₑ ρₛ (patt_total_function f (@patt_sort s₁) (@patt_sort s₂)) = Full ->
       ∀ (m₁ : Domain M),
-        Minterp_inhabitant s₁ ρₑ ρₛ m₁ ->                 
+        Minterp_inhabitant (@patt_sort s₁) ρₑ ρₛ m₁ ->                 
         ∃ (m₂ : Domain M),
-          Minterp_inhabitant s₂ ρₑ ρₛ m₂ ->
+          Minterp_inhabitant (@patt_sort s₂) ρₑ ρₛ m₂ ->
           app_ext (@pattern_interpretation sig M ρₑ ρₛ f) (Ensembles.Singleton (Domain M) m₁)
           = Ensembles.Singleton (Domain M) m₂.
     Proof.
       intros Hfun m₁ H1.
       unfold patt_total_function in Hfun.
+      rewrite -> pattern_interpretation_forall_of_sort_predicate in Hfun.
+      specialize (Hfun m₁ H1).
     Abort.
 
   End with_model.
